proof of eq_chacha20_more_than_256 almost done (store need to be proved)

proof/crypto_stream/chacha20/ref/ChaCha20_pavx2.ec
@@ -240,40 +240,42 @@ module M = {
   (* more than 256                                                       *)
 
   proc init_x8(key, nonce, counter) = {
-    var st_1 : W32.t Array16.t;
-    var st: W32.t Array16.t Array8.t;
-    st_1 <@ ChaCha20_pref.M.init (key, nonce, counter);
-    st.[0] <- st_1; 
-    st.[1] <- st_1.[12 <- st_1.[12] + W32.of_int 1];
-    st.[2] <- st_1.[12 <- st_1.[12] + W32.of_int 2];
-    st.[3] <- st_1.[12 <- st_1.[12] + W32.of_int 3];
-    st.[4] <- st_1.[12 <- st_1.[12] + W32.of_int 4];
-    st.[5] <- st_1.[12 <- st_1.[12] + W32.of_int 5];
-    st.[6] <- st_1.[12 <- st_1.[12] + W32.of_int 6];
-    st.[7] <- st_1.[12 <- st_1.[12] + W32.of_int 7];
-    return st; 
+    var st1, st2, st3, st4, st5, st6, st7, st8 : W32.t Array16.t;
+    st1 <@ ChaCha20_pref.M.init (key, nonce, counter);
+    st2 <- st1.[12 <- st1.[12] + W32.of_int 1];
+    st3 <- st1.[12 <- st1.[12] + W32.of_int 2];
+    st4 <- st1.[12 <- st1.[12] + W32.of_int 3];
+    st5 <- st1.[12 <- st1.[12] + W32.of_int 4];
+    st6 <- st1.[12 <- st1.[12] + W32.of_int 5];
+    st7 <- st1.[12 <- st1.[12] + W32.of_int 6];
+    st8 <- st1.[12 <- st1.[12] + W32.of_int 7];
+    return (st1, st2, st3, st4, st5, st6, st7, st8); 
   }
 
-  proc sum_states_x8(k st: W32.t Array16.t Array8.t) = {
-    var i: int;
-    i <- 0;
-    while (i < 8) {
-      k.[i] <@ ChaCha20_pref.M.sum_states(k.[i], st.[i]);
-      i <- i + 1;
-    }
-    return k;
+  proc sum_states_x8(k1 k2 k3 k4 k5 k6 k7 k8 st1 st2 st3 st4 st5 st6 st7 st8: W32.t Array16.t) = {
+    k1 <@ ChaCha20_pref.M.sum_states(k1, st1);
+    k2 <@ ChaCha20_pref.M.sum_states(k2, st2);
+    k3 <@ ChaCha20_pref.M.sum_states(k3, st3);
+    k4 <@ ChaCha20_pref.M.sum_states(k4, st4);
+    k5 <@ ChaCha20_pref.M.sum_states(k5, st5);
+    k6 <@ ChaCha20_pref.M.sum_states(k6, st6);
+    k7 <@ ChaCha20_pref.M.sum_states(k7, st7);
+    k8 <@ ChaCha20_pref.M.sum_states(k8, st8);
+    return (k1,k2,k3,k4,k5,k6,k7,k8);
   }
 
-  proc increment_counter_x8(st: W32.t Array16.t Array8.t) = {
-    var i: int;
-    i <- 0;
-    while (i < 8) {
-      st.[i] <- st.[i].[12 <- st.[i].[12] + W32.of_int 8];
-      i <- i + 1;
-    }
-    return st;
-  }    
-  
+  proc increment_counter_x8(st1 st2 st3 st4 st5 st6 st7 st8: W32.t Array16.t) = {
+    st1.[12] <- st1.[12] + W32.of_int 8;
+    st2.[12] <- st2.[12] + W32.of_int 8;
+    st3.[12] <- st3.[12] + W32.of_int 8;
+    st4.[12] <- st4.[12] + W32.of_int 8;
+    st5.[12] <- st5.[12] + W32.of_int 8;
+    st6.[12] <- st6.[12] + W32.of_int 8;
+    st7.[12] <- st7.[12] + W32.of_int 8;
+    st8.[12] <- st8.[12] + W32.of_int 8;
+    return (st1, st2, st3, st4, st5, st6, st7, st8); 
+  }
+ 
   proc double_quarter_round_x1_aux (k: W32.t Array16.t, a0 b0 c0 d0 a1 b1 c1 d1 : int) = {
     k <@ ChaCha20_pref.M.quarter_round(k, a0, b0, c0, d0);
     k <@ ChaCha20_pref.M.quarter_round(k, a1, b1, c1, d1);
@@ -354,49 +356,57 @@ module M = {
     return k;
   }
 
-  proc line_x8_v (k: W32.t Array16.t Array8.t , a b c r:int) = {
-    var i:int;
-    i <- 0; 
-    while (i < 8) {
-      k.[i] <@ ChaCha20_pref.M.line(k.[i], a, b, c, r);
-      i <- i + 1;
-    }
-    return k;
+ (* proc line_x8_v (k1 k2 k3 k4 k5 k6 k7 k8: W32.t Array16.t, a b c r:int) = {
+    k1 <@ ChaCha20_pref.M.line(k1, a, b, c, r);
+    k2 <@ ChaCha20_pref.M.line(k2, a, b, c, r);
+    k3 <@ ChaCha20_pref.M.line(k3, a, b, c, r);
+    k4 <@ ChaCha20_pref.M.line(k4, a, b, c, r);
+    k5 <@ ChaCha20_pref.M.line(k5, a, b, c, r);
+    k6 <@ ChaCha20_pref.M.line(k6, a, b, c, r);
+    k7 <@ ChaCha20_pref.M.line(k7, a, b, c, r);
+    k8 <@ ChaCha20_pref.M.line(k8, a, b, c, r);
+    return (k1,k2,k3,k4,k5,k6,k7,k8);
   }
 
-  proc line_2_x8_v (k:W32.t Array16.t Array8.t, a0 b0 c0 r0 a1 b1 c1 r1:int) = {
-    var i:int;
-    i <- 0; 
-    while (i < 8) {
-      k.[i] <@ line_2(k.[i], a0, b0, c0, r0, a1, b1, c1, r1);
-      i <- i + 1;
-    }
-    return k;
+  proc line_2_x8_v (k1 k2 k3 k4 k5 k6 k7 k8:W32.t Array16.t, a0 b0 c0 r0 a1 b1 c1 r1:int) = {
+    k1 <@ line_2(k1, a0, b0, c0, r0, a1, b1, c1, r1);
+    k2 <@ line_2(k2, a0, b0, c0, r0, a1, b1, c1, r1);
+    k3 <@ line_2(k3, a0, b0, c0, r0, a1, b1, c1, r1);
+    k4 <@ line_2(k4, a0, b0, c0, r0, a1, b1, c1, r1);
+    k5 <@ line_2(k5, a0, b0, c0, r0, a1, b1, c1, r1);
+    k6 <@ line_2(k6, a0, b0, c0, r0, a1, b1, c1, r1);
+    k7 <@ line_2(k7, a0, b0, c0, r0, a1, b1, c1, r1);
+    k8 <@ line_2(k8, a0, b0, c0, r0, a1, b1, c1, r1);
+    return (k1,k2,k3,k4,k5,k6,k7,k8);
+  }*)
+
+  proc double_quarter_round_x8 (k1 k2 k3 k4 k5 k6 k7 k8:W32.t Array16.t, a0 b0 c0 d0 a1 b1 c1 d1 : int) = {
+    (k1,k2,k3,k4,k5,k6,k7,k8) <@ line_x1_8  (k1,k2,k3,k4,k5,k6,k7,k8, a0, b0, d0, 16);
+    (k1,k2,k3,k4,k5,k6,k7,k8) <@ line_2_x1_8(k1,k2,k3,k4,k5,k6,k7,k8, c0, d0, b0, 12, a1, b1, d1, 16);
+    (k1,k2,k3,k4,k5,k6,k7,k8) <@ line_2_x1_8(k1,k2,k3,k4,k5,k6,k7,k8, a0, b0, d0, 8,  c1, d1, b1, 12);
+    (k1,k2,k3,k4,k5,k6,k7,k8) <@ line_2_x1_8(k1,k2,k3,k4,k5,k6,k7,k8, c0, d0, b0, 7,  a1, b1, d1, 8);
+    (k1,k2,k3,k4,k5,k6,k7,k8) <@ line_x1_8  (k1,k2,k3,k4,k5,k6,k7,k8, c1, d1, b1, 7);
+    return (k1,k2,k3,k4,k5,k6,k7,k8);
   }
 
-  proc double_quarter_round_x8 (k: W32.t Array16.t Array8.t, a0 b0 c0 d0 a1 b1 c1 d1 : int) = {
-    k <@ line_x8_v (k, a0, b0, d0, 16);
-    k <@ line_2_x8_v(k, c0, d0, b0, 12, a1, b1, d1, 16);
-    k <@ line_2_x8_v(k, a0, b0, d0, 8,  c1, d1, b1, 12);
-    k <@ line_2_x8_v(k, c0, d0, b0, 7,  a1, b1, d1, 8);
-    k <@ line_x8_v(k,  c1, d1, b1, 7);
-    return k;
+  proc column_round_x8(k1 k2 k3 k4 k5 k6 k7 k8:W32.t Array16.t) = {
+    (k1,k2,k3,k4,k5,k6,k7,k8) <@ 
+      double_quarter_round_x8(k1,k2,k3,k4,k5,k6,k7,k8, 0, 4, 8,  12,     
+                                                       2, 6, 10, 14);
+    (k1,k2,k3,k4,k5,k6,k7,k8) <@ 
+     double_quarter_round_x8(k1,k2,k3,k4,k5,k6,k7,k8, 1, 5, 9,  13,
+                                                      3, 7, 11, 15);
+    return (k1,k2,k3,k4,k5,k6,k7,k8);
   }
 
-  proc column_round_x8(k: W32.t Array16.t Array8.t) = {
-    k <@ double_quarter_round_x8(k, 0, 4, 8,  12,     
-                                   2, 6, 10, 14);
-    k <@ double_quarter_round_x8(k, 1, 5, 9,  13,
-                                   3, 7, 11, 15);
-    return k;
-  }
-
-  proc diagonal_round_x8(k: W32.t Array16.t Array8.t) = {
-    k <@ double_quarter_round_x8(k, 1, 6, 11, 12,
-                                    0, 5, 10, 15);
-    k <@ double_quarter_round_x8(k, 2, 7, 8, 13,
-                                    3, 4, 9, 14);
-    return k;
+  proc diagonal_round_x8(k1 k2 k3 k4 k5 k6 k7 k8:W32.t Array16.t) = {
+    (k1,k2,k3,k4,k5,k6,k7,k8) <@ 
+      double_quarter_round_x8(k1,k2,k3,k4,k5,k6,k7,k8, 1, 6, 11, 12,
+                                                       0, 5, 10, 15);
+    (k1,k2,k3,k4,k5,k6,k7,k8) <@ 
+      double_quarter_round_x8(k1,k2,k3,k4,k5,k6,k7,k8, 2, 7, 8, 13,
+                                                       3, 4, 9, 14);
+    return (k1,k2,k3,k4,k5,k6,k7,k8);
   }
   
   proc rounds_x1 (k: W32.t Array16.t) = {
@@ -410,43 +420,41 @@ module M = {
     return k;
   }
 
-  proc rounds_x8 (k: W32.t Array16.t Array8.t) = {
+  proc rounds_x8 (k1 k2 k3 k4 k5 k6 k7 k8:W32.t Array16.t) = {
     var c : int;
     c <- 0;
     while (c < 10) {
-      k <@ column_round_x8(k);
-      k <@ diagonal_round_x8(k);
+      (k1,k2,k3,k4,k5,k6,k7,k8) <@ column_round_x8(k1,k2,k3,k4,k5,k6,k7,k8);
+      (k1,k2,k3,k4,k5,k6,k7,k8) <@ diagonal_round_x8(k1,k2,k3,k4,k5,k6,k7,k8);
       c <- c + 1;
     }
-    return k;
+    return (k1,k2,k3,k4,k5,k6,k7,k8);
   }
 
-  proc body_x8 (st: W32.t Array16.t Array8.t) = {
-    var k: W32.t Array16.t Array8.t;
-    k <@ rounds_x8(st);
-    k <@ sum_states_x8(k, st);
-    st <@ increment_counter_x8(st);
-    return (k, st);
+  proc body_x8 (st1 st2 st3 st4 st5 st6 st7 st8: W32.t Array16.t) = {
+    var k1,k2,k3,k4,k5,k6,k7,k8: W32.t Array16.t;
+    (k1,k2,k3,k4,k5,k6,k7,k8) <@ rounds_x8(st1,st2,st3,st4,st5,st6,st7,st8);
+    (k1,k2,k3,k4,k5,k6,k7,k8) <@ sum_states_x8(k1,k2,k3,k4,k5,k6,k7,k8, st1,st2,st3,st4,st5,st6,st7,st8);
+    (st1,st2,st3,st4,st5,st6,st7,st8) <@ increment_counter_x8(st1,st2,st3,st4,st5,st6,st7,st8);
+    return (k1,k2,k3,k4,k5,k6,k7,k8, st1,st2,st3,st4,st5,st6,st7,st8);
   }
 
   proc chacha20_more_than_256(output plain len: int, key nonce: int, counter:W32.t) : unit = {
-    var st, k: W32.t Array16.t Array8.t;
+    var k1,k2,k3,k4,k5,k6,k7,k8, st1,st2,st3,st4,st5,st6,st7,st8: W32.t Array16.t;
     
-    st <@ init_x8(key, nonce, counter);
+    (st1,st2,st3,st4,st5,st6,st7,st8) <@ init_x8(key, nonce, counter);
 
     while( 512 <= len) {
-      k <@ rounds_x8(st);
-      k <@ sum_states_x8(k, st);
-      (output, plain, len) <@ ChaCha20_pavx2_cf.M.store_x8(output, plain, len, k.[0], k.[1], k.[2], k.[3],
-                                                                              k.[4], k.[5], k.[6], k.[7]);
-      st <@ increment_counter_x8(st);
+      (k1,k2,k3,k4,k5,k6,k7,k8) <@ rounds_x8(st1,st2,st3,st4,st5,st6,st7,st8);
+      (k1,k2,k3,k4,k5,k6,k7,k8) <@ sum_states_x8(k1,k2,k3,k4,k5,k6,k7,k8, st1,st2,st3,st4,st5,st6,st7,st8);
+      (output, plain, len) <@ ChaCha20_pavx2_cf.M.store_x8(output, plain, len, k1,k2,k3,k4,k5,k6,k7,k8);
+      (st1,st2,st3,st4,st5,st6,st7,st8) <@ increment_counter_x8(st1,st2,st3,st4,st5,st6,st7,st8);
     }
 
     if(0 < len) {
-      k <@ rounds_x8(st);
-      k <@ sum_states_x8(k, st);
-      ChaCha20_pavx2_cf.M.store_x8_last(output, plain, len, k.[0], k.[1], k.[2], k.[3],
-                                                      k.[4], k.[5], k.[6], k.[7]);
+      (k1,k2,k3,k4,k5,k6,k7,k8) <@ rounds_x8(st1,st2,st3,st4,st5,st6,st7,st8);
+      (k1,k2,k3,k4,k5,k6,k7,k8) <@ sum_states_x8(k1,k2,k3,k4,k5,k6,k7,k8, st1,st2,st3,st4,st5,st6,st7,st8);
+      ChaCha20_pavx2_cf.M.store_x8_last(output, plain, len, k1,k2,k3,k4,k5,k6,k7,k8);
     }
   }
 
@@ -625,94 +633,64 @@ proof.
   move=> &2; split; ring.
 qed.
 
-op is_incr_count8 (st1: W32.t Array16.t) (st2: W32.t Array16.t Array8.t) = 
-   st2 = Array8.init (fun i => st1.[12 <- st1.[12] + W32.of_int i]).
+op is_incr_count8 (st: W32.t Array16.t) (st1 st2 st3 st4 st5 st6 st7 st8: W32.t Array16.t) = 
+   st1 = st /\
+   st2 = st.[12 <- st.[12] +  W32.of_int 1] /\
+   st3 = st.[12 <- st.[12] +  W32.of_int 2] /\
+   st4 = st.[12 <- st.[12] +  W32.of_int 3] /\
+   st5 = st.[12 <- st.[12] +  W32.of_int 4] /\
+   st6 = st.[12 <- st.[12] +  W32.of_int 5] /\
+   st7 = st.[12 <- st.[12] +  W32.of_int 6] /\
+   st8 = st.[12 <- st.[12] +  W32.of_int 7].
 
-equiv eq_line_x1_x8 :
-   M.line_x1_8 ~ M.line_x8_v :
-   ={a,b,c,r} /\
-   k{2} = Array8.of_list witness 
-            [k1{1}; k2{1}; k3{1}; k4{1}; k5{1}; k6{1}; k7{1}; k8{1}] ==>
-   res{2} = 
-     Array8.of_list witness 
-      [res{1}.`1; res{1}.`2; res{1}.`3; res{1}.`4; res{1}.`5; res{1}.`6; res{1}.`7; res{1}.`8].
-proof.
-  proc => /=. 
-  conseq (_: Array8.all_eq k{2} 
-             (Array8.of_list witness [k1{1}; k2{1}; k3{1}; k4{1}; k5{1}; k6{1}; k7{1}; k8{1}])).
-  + by move=> *;apply Array8.all_eq_eq.
-  unroll for{2} ^while.
-  by do !(wp; call (_:true) => /=; 1: by sim); wp; skip.
-qed.
+equiv eq_line : ChaCha20_pref.M.line ~ ChaCha20_pref.M.line :
+   ={k, a, b, c, r} ==> ={res}.
+proof. by sim. qed.
 
-equiv eq_line_2_x1_x8 :
-   M.line_2_x1_8 ~ M.line_2_x8_v :
-  ={a0,b0,c0,r0, a1,b1,c1,r1} /\
-   k{2} = Array8.of_list witness 
-            [k1{1}; k2{1}; k3{1}; k4{1}; k5{1}; k6{1}; k7{1}; k8{1}] ==>
-   res{2} = 
-     Array8.of_list witness 
-      [res{1}.`1; res{1}.`2; res{1}.`3; res{1}.`4; res{1}.`5; res{1}.`6; res{1}.`7; res{1}.`8].
-proof.
-  proc => /=. 
-  conseq (_: Array8.all_eq k{2} 
-             (Array8.of_list witness [k1{1}; k2{1}; k3{1}; k4{1}; k5{1}; k6{1}; k7{1}; k8{1}])).
-  + by move=> *;apply Array8.all_eq_eq.
-  unroll for{2} ^while.
-  by do !(wp; call (_:true) => /=; 1: by sim); wp; skip.
-qed.
+equiv eq_line_2 : M.line_2 ~ M.line_2 :
+   ={k, a0, b0, c0, r0, a1, b1, c1, r1} ==> ={res}.
+proof. by sim. qed.
 
 equiv eq_double_quarter_round_x1_x8 :
    M.double_quarter_round_x1_8 ~ M.double_quarter_round_x8 :
-   ={a0,b0,c0,d0, a1,b1,c1,d1} /\
-   k{2} = Array8.of_list witness 
-            [k1{1}; k2{1}; k3{1}; k4{1}; k5{1}; k6{1}; k7{1}; k8{1}] ==>
-   res{2} = 
-     Array8.of_list witness 
-      [res{1}.`1; res{1}.`2; res{1}.`3; res{1}.`4; res{1}.`5; res{1}.`6; res{1}.`7; res{1}.`8].
+   ={a0,b0,c0,d0, a1,b1,c1,d1, k1,k2,k3,k4,k5,k6,k7,k8}
+   ==>
+   ={res}.
 proof.
   proc => /=.
   inline M.double_quarter_round_x1.
   interleave{1} [1:9] [16:9] [31:9] [46:9] [61:9] [76:9] [91:9] [106:9] 1 .
   interleave{1} [73:1] [79:1] [85:1] [91:1] [97:1] [103:1] [109:1] [115:1] 5.
   wp.
-  replace * {1} { [1..72]! _ as c; _ <@_; _} by {
-    c;
-    (k, k0, k9, k10, k11, k12, k13, k14) <@ 
-       M.line_x1_8(k, k0, k9, k10, k11, k12, k13, k14, a0, b0, d0, 16);
-    (k, k0, k9, k10, k11, k12, k13, k14) <@
-       M.line_2_x1_8(k, k0, k9, k10, k11, k12, k13, k14, c0, d0, b0, 12, a1, b1, d1, 16); 
-    (k, k0, k9, k10, k11, k12, k13, k14) <@
-       M.line_2_x1_8(k, k0, k9, k10, k11, k12, k13, k14, a0, b0, d0, 8, c1, d1, b1, 12);
-    (k, k0, k9, k10, k11, k12, k13, k14) <@
-       M.line_2_x1_8(k, k0, k9, k10, k11, k12, k13, k14, c0, d0, b0, 7, a1, b1, d1, 8);
-    (k, k0, k9, k10, k11, k12, k13, k14) <@
-       M.line_x1_8(k, k0, k9, k10, k11, k12, k13, k14, c1, d1, b1, 7);
-  }. + smt(). + done.
-  + inline M.line_x1_8 M.line_2_x1_8.
-    by do !(wp;call (_:true) => /=; 1:by sim);wp; skip => />.
-  call eq_line_x1_x8; do 3! call eq_line_2_x1_x8; call eq_line_x1_x8; wp; skip => />.
+  inline{2} M.line_x1_8 M.line_2_x1_8. 
+  wp; do !(call eq_line); wp => /=.
+  do !(do !call eq_line_2; wp => /=).
+  do !(call eq_line); wp => /=; skip => />.
 qed.
 
 equiv eq_body_x8 : ChaCha20_pavx2_cf.M.body_x8 ~ M.body_x8 : 
-   is_incr_count8 st_1{1} st{2} ==>
-   is_incr_count8 res{1}.`1 res{2}.`2 /\
-   res{2}.`1 = Array8.of_list witness [res{1}.`2; res{1}.`3; res{1}.`4; res{1}.`5;
-                                       res{1}.`6; res{1}.`7; res{1}.`8; res{1}.`9].
+   is_incr_count8 st_1{1} st1{2} st2{2} st3{2} st4{2} st5{2} st6{2} st7{2} st8{2} ==>
+   is_incr_count8 res{1}.`1 
+    res{2}.`9 res{2}.`10 res{2}.`11 res{2}.`12 res{2}.`13 res{2}.`14 res{2}.`15 res{2}.`16 /\
+   res{1}.`2 = res{2}.`1 /\
+   res{1}.`3 = res{2}.`2 /\
+   res{1}.`4 = res{2}.`3 /\
+   res{1}.`5 = res{2}.`4 /\
+   res{1}.`6 = res{2}.`5 /\
+   res{1}.`7 = res{2}.`6 /\
+   res{1}.`8 = res{2}.`7 /\
+   res{1}.`9 = res{2}.`8.
 proof.
   proc => /=.
   swap{1} 3 -2, {1} 6 -4, {1} 9 -6, {1} 12 -8, {1} 15 -10, {1} 18 -12, {1} 21 -14. 
   interleave{1} [8:1] [10:1] [12:1] [14:1] [16:1] [18:1] [20:1] [22:1] 2.
-  seq 7 0 : (is_incr_count8 st_1{1} st{2} /\
-             st{2} = Array8.of_list witness [st_1{1}; st_2{1}; st_3{1}; st_4{1}; 
-                                             st_5{1}; st_6{1}; st_7{1}; st_8{1} ]).
-  + conseq (_:Array8.all_eq st{2} (Array8.of_list witness [st_1{1}; st_2{1}; st_3{1}; st_4{1}; 
-                                                           st_5{1}; st_6{1}; st_7{1}; st_8{1} ])).
-    + by move=> |> *;apply Array8.all_eq_eq.
-    inline ChaCha20_pref.M.increment_counter;wp; skip; rewrite /Array8.all_eq /= /is_incr_count8.
-    by move=> &1 &2 -> /=; rewrite set_notmod.
-  seq 8 1 : (#pre /\ k{2} = Array8.of_list witness [k_1{1}; k_2{1}; k_3{1}; k_4{1}; 
-                                                    k_5{1}; k_6{1}; k_7{1}; k_8{1} ]).
+  seq 7 0 : (is_incr_count8 st_1{1} st1{2} st2{2} st3{2} st4{2} st5{2} st6{2} st7{2} st8{2} /\
+             st_1{1} = st1{2} /\ st_2{1} = st2{2} /\ st_3{1} = st3{2} /\ st_4{1} = st4{2} /\ 
+             st_5{1} = st5{2} /\ st_6{1} = st6{2} /\ st_7{1} = st7{2} /\ st_8{1} = st8{2}).
+  + by inline ChaCha20_pref.M.increment_counter;wp; skip; rewrite /is_incr_count8 => />.
+  seq 8 1 : (#pre /\ 
+             k_1{1} = k1{2} /\ k_2{1} = k2{2} /\ k_3{1} = k3{2} /\ k_4{1} = k4{2} /\
+             k_5{1} = k5{2} /\ k_6{1} = k6{2} /\ k_7{1} = k7{2} /\ k_8{1} = k8{2}).
   + conseq |>.
     transitivity*{1} {
       k_1 <@ M.rounds_x1(st_1);
@@ -752,7 +730,6 @@ proof.
     }. + smt(). + done.
     + interleave{1} [1:1] [5:1] [9:1] [13:1] [17:1] [21:1] [25:1] [29:1] 1.
       interleave{1} [9:2] [12:2] [15:2] [18:2] [21:2] [24:2] [27:2] [30:2] 1.
-
       wp; do 8! unroll for{1} ^while.
       interleave{1} [9:3] [40:3] [71:3] [102:3] [133:3] [164:3] [195:3] [226:3] 10.
       by unroll for{2} ^while; sim.
@@ -790,13 +767,8 @@ proof.
       by do !(wp; call (_:true) => /=; 1: by sim); wp; skip => />.
     by do 2! call eq_double_quarter_round_x1_x8; skip.
   seq 8 1 : (#pre).  
-  + conseq />; inline M.sum_states_x8.      
-    unroll for{2} ^while.
-    do !(wp; call (_:true) =>/=;1: by sim); wp; skip => />.
-    by move=> &1 ? 8?; apply Array8.all_eq_eq.
-  conseq />; inline *; rewrite /is_incr_count8.
-  unroll for{2} ^while; wp; skip=> &1 &2 [#] -> /Array8.ext_eq_all /> ?.
-  by apply Array8.all_eq_eq; rewrite /Array8.all_eq /=.
+  + by conseq />; inline M.sum_states_x8; sim.  
+  by conseq />; inline *; wp; skip; rewrite /is_incr_count8 => />.
 qed.
 
 equiv eq_chacha20_more_than_256 : ChaCha20_pavx2_cf.M.chacha20_more_than_256 ~ M.chacha20_more_than_256 :
@@ -804,31 +776,31 @@ equiv eq_chacha20_more_than_256 : ChaCha20_pavx2_cf.M.chacha20_more_than_256 ~ M
    ={Glob.mem}.
 proof.
   proc => /=.
-  seq 1 1 : (={output, plain, len, Glob.mem} /\ is_incr_count8 st_1{1} st{2}).
+  seq 1 1 : (={output, plain, len, Glob.mem} /\ 
+             is_incr_count8 st_1{1} st1{2} st2{2} st3{2} st4{2} st5{2} st6{2} st7{2} st8{2}).
   + conseq />; inline M.init_x8; wp.
     call (_: ={Glob.mem}); 1: by sim.
-    wp; skip => />.
-    move=> &2 st; rewrite /is_incr_count8.
-    by apply Array8.all_eq_eq => />; rewrite set_notmod.
+    by wp; skip => />.
   transitivity* {2} {
     while (512 <= len) {                          
-      (k,st) <@ M.body_x8(st);
+      (k1, k2, k3, k4, k5, k6, k7, k8, st1, st2, st3, st4, st5, st6, st7, st8) <@ 
+        M.body_x8(st1, st2, st3, st4, st5, st6, st7, st8);
       (output, plain, len) <@ ChaCha20_pavx2_cf.M.store_x8(output, plain, len, 
-                                                          k.[0], k.[1], k.[2], k.[3], 
-                                                          k.[4], k.[5], k.[6], k.[7]);
+                                                           k1, k2, k3, k4, k5, k6, k7, k8);
     }
     if (0 < len) {   
-      (k,st) <@ M.body_x8(st);                                  
-      ChaCha20_pavx2_cf.M.store_x8_last(output, plain, len, k.[0], k.[1], k.[2], k.[3], 
-                                                     k.[4], k.[5], k.[6], k.[7]);
+      (k1, k2, k3, k4, k5, k6, k7, k8, st1, st2, st3, st4, st5, st6, st7, st8) <@ 
+        M.body_x8(st1, st2, st3, st4, st5, st6, st7, st8);                                  
+      ChaCha20_pavx2_cf.M.store_x8_last(output, plain, len,
+                                        k1, k2, k3, k4, k5, k6, k7, k8);
     }
   }; [1:smt () |2: done]; last first.
   + seq 1 1 : (#pre).
     + while (#pre); last by auto.
-      inline [-tuple] M.body_x8. 
-      by swap{1} 4 1, {1}[5..6] 1, {1} [6..8] 1; sim.
+      inline [-tuple] M.body_x8.  
+      by swap{2} 3 1; sim.
     if => //.
-    by inline [-tuple] M.increment_counter_x8 M.body_x8; unroll for{1} ^while; sim.
+    by inline [-tuple] M.increment_counter_x8 M.body_x8; sim. 
   seq 1 1 : (#pre).
   + while (#pre); last by auto.
     call (_: ={Glob.mem}) => /=; 1:sim. 
